Generalized wf_red with error cases.

Semantics.v
@@ -10,7 +10,7 @@ License: MIT.
 *)
 
 Set Implicit Arguments.
-Require Export Typing Validity.
+Require Export Typing.
 
 Open Scope set_scope.
 Open Scope container_scope.
@@ -59,7 +59,6 @@ Inductive uninitialized (C:typdefctx) : typ -> val -> Prop :=
   | uninitialized_double :
       uninitialized C typ_double val_uninitialized
   | uninitialized_ptr : forall T,
-      (* wf_typ C T -> *)
       uninitialized C (typ_ptr T) val_uninitialized
   | uninitialized_array : forall os T Ta a,
       typing_array C Ta T os ->
@@ -173,9 +172,9 @@ Inductive red (C:typdefctx) :  stack -> state -> trm -> state -> val -> Prop :=
       vr = val_abstract_ptr l nil ->
       l <> null ->
       l \notindom m1 ->
-      valid_typ C T ->
+      wf_typ C T ->
       uninitialized C T v -> 
-      m2 = m1[l := v] ->
+      m2 = m1[l:=v] ->
       red C S m1 (trm_app (prim_new T) nil) m2 vr
   | red_new_array : forall l (n:int) (k:nat) a S m1 T v1 m2 vr,
       v1 = val_int n ->
@@ -183,9 +182,9 @@ Inductive red (C:typdefctx) :  stack -> state -> trm -> state -> val -> Prop :=
       l <> null ->
       l \notindom m1 ->
       n = k ->
-      valid_typ C T ->
+      wf_typ C T ->
       uninitialized C (typ_array T (Some k)) (val_array (typ_array T (Some k)) a) -> 
-      m2 = m1[l := (val_array (typ_array T None) a)] ->
+      m2 = m1[l:=(val_array (typ_array T None) a)] ->
       red C S m1 (trm_app (prim_new_array T) ((trm_val v1)::nil)) m2 vr
   | red_struct_access : forall l π S T f v1 m vr,
       v1 = val_abstract_ptr l π ->
@@ -250,11 +249,11 @@ Inductive red (C:typdefctx) :  stack -> state -> trm -> state -> val -> Prop :=
   | red_new_error : forall S T m,
       ~ (exists v, uninitialized C T v) ->
       red C S m (trm_app (prim_new T) nil) m val_error
-  | red_new_array_error : forall (n:int) (k:nat) S m1 T v1 m2,
+  | red_new_array_error : forall (n:int) (k:nat) S m T v1,
       v1 = val_int n ->
       n = k ->
       ~ (exists a, uninitialized C (typ_array T (Some k)) (val_array (typ_array T (Some k)) a)) -> 
-      red C S m1 (trm_app (prim_new_array T) ((trm_val v1)::nil)) m2 val_error
+      red C S m (trm_app (prim_new_array T) ((trm_val v1)::nil)) m val_error
   | red_struct_access_error_not_a_ptr : forall S T f v1 m,
       ~ is_ptr v1 ->
       red C S m (trm_app (prim_struct_access T f) ((trm_val v1)::nil)) m val_error
@@ -345,8 +344,10 @@ Lemma not_is_error_args_1 : forall C S m op ts m' v w,
   ~ is_error v ->
   ~ is_error w.
 Proof.
-  introv HR He HN. destruct w; inverts HN;
-  inverts HR; tryfalse*. inverts_head red; tryfalse*.
+  introv HR He HN. destruct w; try inverts HN.
+  destruct b; inverts HN.
+  inverts HR; tryfalse*.
+  inverts_head red; tryfalse*.
 Qed.
 
 Lemma not_is_error_args_2 : forall C S m op t ts m' v w,
@@ -354,8 +355,10 @@ Lemma not_is_error_args_2 : forall C S m op t ts m' v w,
   ~ is_error v ->
   ~ is_error w.
 Proof.
-  introv HR He HN. destruct w; inverts HN; 
-  inverts HR; tryfalse*. inverts_head red; tryfalse*.
+  introv HR He HN. destruct w; try inverts HN.
+  destruct b; inverts HN.
+  inverts HR; tryfalse*.
+  inverts_head red; tryfalse*.
 Qed.
 
 
@@ -370,34 +373,22 @@ Admitted.
 
 
 (* ********************************************************************** *)
-(* * Validity results *)
+(* * Results of the connection between semantics and well-foundedness. *)
 
-Lemma stack_valid_add : forall C x v S,
-  valid_stack C S ->
-  valid_val C v ->
-  valid_stack C (Ctx.add x v S).
-Proof.
-  introv HS Hv. unfolds Ctx.add. destruct~ x.
-  unfolds. introv HCl. unfold Ctx.lookup in HCl.
-  case_if in HCl.
-  { inverts~ HCl. }
-  { applys~ HS x. }
-Qed.
-
-Lemma redbinop_valid : forall op v1 v2 C vr,
+Lemma wf_redbinop : forall op v1 v2 C vr,
   redbinop op v1 v2 vr ->
-  valid_val C v1 ->
-  valid_val C v2 ->
-  valid_val C vr.
+  wf_val C v1 ->
+  wf_val C v2 ->
+  wf_val C vr.
 Proof.
   introv HR Hv1 Hv2. induction HR; constructors*.
 Qed.
 
-Lemma read_accesses_valid : forall v1 π C v2,
+Lemma wf_read_accesses : forall v1 π C v2,
   read_accesses v1 π v2 ->
-  valid_val C v1 ->
-  valid_accesses C π ->
-  valid_val C v2.
+  wf_val C v1 ->
+  wf_accesses C π ->
+  wf_val C v2.
 Proof.
   introv HR Hv1 Hπ. induction HR.
   { auto. }
@@ -407,22 +398,22 @@ Proof.
     applys~ IHHR. }
 Qed.
 
-Lemma read_state_valid : forall m l π C v,
+Lemma wf_read_state : forall m l π C v,
   read_state m l π v ->
-  valid_state C m ->
-  valid_accesses C π ->
-  valid_val C v.
+  wf_state C m ->
+  wf_accesses C π ->
+  wf_val C v.
 Proof.
-  introv HR Hm Hπ. unfolds valid_state. inverts HR.
-  forwards*: Hm. applys* read_accesses_valid.
+  introv HR Hm Hπ. unfolds wf_state. inverts HR.
+  forwards*: Hm. applys* wf_read_accesses.
 Qed.
 
-Lemma write_accesses_valid : forall v1 w π C v2,
+Lemma wf_write_accesses : forall v1 w π C v2,
   write_accesses v1 π w v2 ->
-  valid_val C v1 ->
-  valid_val C w ->
-  valid_accesses C π ->
-  valid_val C v2.
+  wf_val C v1 ->
+  wf_val C w ->
+  wf_accesses C π ->
+  wf_val C v2.
 Proof.
   introv HW Hv1 Hw Hπ. induction HW.
   { auto. }
@@ -432,114 +423,109 @@ Proof.
     constructors*. introv Hf. rew_reads*. }
 Qed.
 
-Lemma write_state_valid : forall m1 l π v C m2,
+Lemma wf_write_state : forall m1 l π v C m2,
   write_state m1 l π v m2 ->
-  valid_state C m1 ->
-  valid_accesses C π ->
-  valid_val C v ->
-  valid_state C m2.
-Proof. 
-  introv HW Hm1 Hπ Hv. inverts HW. unfolds valid_state.
+  wf_state C m1 ->
+  wf_accesses C π ->
+  wf_val C v ->
+  wf_state C m2.
+Proof.
+  introv HW Hm1 Hπ Hv. inverts HW. unfolds wf_state.
   forwards*: Hm1. introv Hl0. rew_reads*; intros.
-  { applys* write_accesses_valid. }
+  { applys* wf_write_accesses. }
   { applys~ Hm1. applys~ indom_update_inv_neq l l0 v2. }
 Qed.
 
-Lemma typing_array_valid : forall Ta os C T,
-  typing_array C Ta T os ->
-  valid_typ C Ta ->
-  valid_typ C T.
-Proof.
-  introv HTa HVTa. induction HTa; inverts~ HVTa.
-Qed.
-
-Lemma typing_struct_valid : forall Ts C Tfs,
-  typing_struct C Ts Tfs ->
-  valid_typ C Ts ->
-  (forall f,
-    f \indom Tfs ->
-    valid_typ C Tfs[f]).
-Proof.
-  introv HTs HVTs. induction HTs; inverts~ HVTs.
-Qed.
-
-Lemma uninitialized_valid : forall v C T,
-  valid_typ C T ->
+Lemma wf_uninitialized : forall v C T,
+  wf_typ C T ->
   uninitialized C T v ->
-  valid_val C v.
+  wf_val C v.
 Proof.
   introv HT Hu. induction Hu; try solve [ constructors* ].
   { constructors~. introv Hi. applys~ H2.
-    applys* typing_array_valid. }
+    applys* wf_typing_array. }
   { constructors~. introv Hf. rewrite <- H0 in Hf. applys~ H2.
-    applys* typing_struct_valid. }
+    applys* wf_typing_struct. }
 Qed.
 
 (* Path surgery of valid accesses *)
 
-Lemma valid_accesses_app : forall C π1 π2,
-  valid_accesses C π1 ->
-  valid_accesses C π2 ->
-  valid_accesses C (π1 ++ π2).
+Lemma wf_accesses_app : forall C π1 π2,
+  wf_accesses C π1 ->
+  wf_accesses C π2 ->
+  wf_accesses C (π1 ++ π2).
 Proof.
   introv Ha1 Ha2. gen π2. induction Ha1; intros;
   rew_list in *; eauto; constructors~.
 Qed.
 
-Lemma red_valid : forall S m1 t C m2 v,
+(* Preservation of well-foundedness by the semantics. *)
+
+Lemma wf_red : forall S m1 t C m2 v,
   red C S m1 t m2 v ->
-  valid_stack C S ->
-  valid_state C m1 ->
-  valid_trm C t ->
-  ~ is_error v -> (* TODO: No need to assume this. *)
-      valid_state C m2
-  /\  valid_val C v.
+  wf_stack C S ->
+  wf_state C m1 ->
+  wf_trm C t ->
+      wf_state C m2
+  /\  wf_val C v.
 Proof.
-  introv HR HS Hm1 Ht He. induction HR; intros;
-  try solve [ inverts* Ht ; forwards*: He ].
-  { inverts Ht. forwards* (Hm2&HVb): IHHR1.
+  introv HR HS Hm1 Ht. induction HR; intros;
+  try solve [ inverts Ht ; splits* ; constructors* ].
+  { (* if *)
+    inverts Ht. forwards* (Hm2&HVb): IHHR1.
     applys~ IHHR2. case_if*. }
-  { inverts Ht. forwards* (Hm2&HVb): IHHR1.
-    applys~ IHHR2. applys~ stack_valid_add. }
-  { inverts Ht as Hop Hv1 Hv2.
+  { (* let *)
+    inverts Ht. forwards* (Hm2&HVb): IHHR1.
+    applys~ IHHR2. applys~ wf_stack_add. }
+  { (* binop *)
+    inverts Ht as Hop Hv1 Hv2.
     inverts Hv1 as Hv1. inverts Hv2 as Hv2.
-    splits~. applys* redbinop_valid. }
-  { subst. inverts Ht as Hop Hp. inverts Hp as Hp. 
-    inverts Hp as Hπ. splits~. 
-    applys* read_state_valid. }
-  { subst. inverts Ht as Hop Hp Hv2. 
+    splits~. applys* wf_redbinop. }
+  { (* get *)
+    subst. inverts Ht as Hop Hp. inverts Hp as Hp. 
+    inverts Hp as Hπ. splits~.
+    applys* wf_read_state. }
+  { (* set *)
+    subst. inverts Ht as Hop Hp Hv2. 
     inverts Hv2 as Hv2. inverts Hp as Hp.
     inverts Hp as Hπ. splits; try constructors*.
-    applys* write_state_valid. }
-  { subst. splits.
-    { unfolds valid_state. introv Hl0. rew_reads; intros; subst.
-      { applys* uninitialized_valid. }
+    applys* wf_write_state. }
+  { (* new *)
+    subst. splits.
+    { unfolds wf_state. introv Hl0. rew_reads; intros; subst.
+      { applys* wf_uninitialized. }
       { applys~ Hm1. applys~ indom_update_inv_neq l l0 v. } }
     { repeat constructors*. } }
-  { subst. splits.
-    { unfolds valid_state. introv Hl0. rew_reads; intros; subst.
-      { forwards HV: uninitialized_valid H5. { constructors~. }
+  { (* new_array *)
+    subst. splits.
+    { unfolds wf_state. introv Hl0. rew_reads; intros; subst.
+      { forwards* HV: wf_uninitialized H5. 
+        { constructors~. }
         inverts HV as HV HVai. repeat constructors~. }
       { applys~ Hm1. applys* indom_update_inv_neq l l0. } }
     { repeat constructors*. } }
-  { subst. inverts Ht as Hop Hp. inverts Hop. inverts Hp as Hπ.
-    splits~. constructors~. inverts Hπ. applys~ valid_accesses_app.
+  { (* struct_access *)
+    subst. inverts Ht as Hop Hp. inverts Hop. inverts Hp as Hπ.
+    splits~. constructors~. inverts Hπ. applys~ wf_accesses_app.
     repeat constructors~. }
-  { subst. inverts Ht as Hop Hp Hi. inverts Hop. inverts Hp as Hπ.
-    splits~. constructors~. inverts Hπ. applys~ valid_accesses_app.
+  { (* array_access *)
+    subst. inverts Ht as Hop Hp Hi. inverts Hop. inverts Hp as Hπ.
+    splits~. constructors~. inverts Hπ. applys~ wf_accesses_app.
     repeat constructors~. }
-  { subst. inverts Ht as Hop Hs. inverts Hop. inverts Hs as Hs.
+  { (* struct_get *)
+    subst. inverts Ht as Hop Hs. inverts Hop. inverts Hs as Hs.
     inverts Hs as Hs Hsf0. splits~. }
-  { subst. inverts Ht as Hop Ha Hi. inverts Ha as Ha.
+  { (* array_get *)
+    subst. inverts Ht as Hop Ha Hi. inverts Ha as Ha.
     inverts Ha as Ha Hai. splits~. }
-  { forwards* (Hm2&Hv1): IHHR1.
+  { (* args_1 *)
+    forwards* (Hm2&Hv1): IHHR1.
     { inverts~ Ht. }
-    { applys* not_is_error_args_1. }
     applys~ IHHR2.
     { inverts~ Ht; repeat constructors~. } }
-  { forwards* (Hm2&Hv1): IHHR1.
+  { (* args_2 *)
+    forwards* (Hm2&Hv1): IHHR1.
     { inverts~ Ht. }
-    { applys* not_is_error_args_2. }
     applys~ IHHR2.
     { inverts~ Ht; repeat constructors~. } }
 Qed.
